x

formal-verification/FormalVerification/SemanticEquivalence/Insertion.lean
@@ -16,6 +16,96 @@ open SemaphoreMTB (F Order)
 open SemaphoreMTB renaming InsertionRound_30_30 → gInsertionRound
 open SemaphoreMTB renaming InsertionProof_4_30_4_4_30 → gInsertionProof
 
+lemma MerkleTree.item_at_nat_to_fin' {depth : Nat} {F: Type} {H: Hash F 2} (t : MerkleTree F H depth) (idx : Nat) (h : idx < 2 ^ depth):
+  MerkleTree.item_at_nat t idx = some (MerkleTree.tree_item_at_fin t ⟨idx, h⟩) := by
+  simp [MerkleTree.item_at_nat, MerkleTree.tree_item_at_fin]
+  simp [Dir.nat_to_dir_vec, Dir.fin_to_dir_vec]
+  simp [fin_to_bits_le_is_some h]
+  congr
+  apply Fin.eq_of_veq
+  apply Fin.val_cast_of_lt
+  assumption
+
+lemma nat_to_bits_le_some_when_lt :
+  nat_to_bits_le l a = some w → a < 2 ^ l := by
+  induction l generalizing a with
+  | zero =>
+    unfold nat_to_bits_le
+    split <;> simp [*]
+  | succ l ih =>
+    unfold nat_to_bits_le
+    simp [Bind.bind]
+    intro w h _
+    have := ih h
+    apply Nat.lt_of_div_lt_div (k := 2)
+    simpa [Nat.pow_succ]
+
+lemma MerkleTree.item_at_nat_some_when_le {D : Nat} {tree : MerkleTree α H D}:
+  MerkleTree.item_at_nat tree idx = some el → idx < 2 ^ D := by
+  intro h
+  unfold item_at_nat at h
+  unfold Dir.nat_to_dir_vec at h
+  simp at h
+  rcases h with ⟨a, h, -⟩
+  exact nat_to_bits_le_some_when_lt h
+
+lemma MerkleTree.item_at_nat_none_when_ge {D : Nat} {tree : MerkleTree α H D}:
+  idx ≥ 2^D → MerkleTree.item_at_nat tree idx = none := by
+  intro h
+  cases hp : item_at_nat tree idx
+  . rfl
+  . have := MerkleTree.item_at_nat_some_when_le hp
+    exfalso
+    exact not_lt_of_ge h this
+
+lemma MerkleTree.set_at_nat_some_when_le {D:Nat} {tree tree': MerkleTree α H D}:
+  MerkleTree.set_at_nat tree idx el = some tree' → idx < 2 ^ D := by
+  unfold MerkleTree.set_at_nat
+  unfold Dir.nat_to_dir_vec
+  simp
+  intro w h _
+  exact nat_to_bits_le_some_when_lt h
+
+
+lemma fin_to_bits_le_is_some' {depth : Nat} {idx : Nat} (h : idx < 2 ^ depth) :
+  nat_to_bits_le depth idx = some (fin_to_bits_le ⟨idx, h⟩) := by
+  simp [fin_to_bits_le]
+  split <;> tauto
+
+lemma MerkleTree.set_at_nat_to_fin' {depth : Nat} {F: Type} {H: Hash F 2} (t : MerkleTree F H depth) (idx : Nat) (item : F) (h : idx < 2 ^ depth):
+  MerkleTree.set_at_nat t idx item = some (MerkleTree.tree_set_at_fin t ⟨idx, h⟩ item) := by
+  simp [MerkleTree.set_at_nat, MerkleTree.tree_set_at_fin]
+  simp [Dir.nat_to_dir_vec]
+  simp [Dir.fin_to_dir_vec]
+  simp [fin_to_bits_le_is_some' h]
+
+lemma MerkleTree.set_at_nat_to_fin_some' {depth : Nat} {F: Type} {H: Hash F 2} {a : MerkleTree F H depth} (t : MerkleTree F H depth) (idx : Nat) (item : F) (h : idx < 2 ^ depth):
+  MerkleTree.set_at_nat t idx item = some a ↔
+  MerkleTree.tree_set_at_fin t ⟨idx, h⟩ item = a := by
+  rw [set_at_nat_to_fin' (h := h)]
+  simp
+
+lemma MerkleTree.item_at_nat_to_fin_some' {depth : Nat} {F: Type} {H: Hash F 2} {a : F} (t : MerkleTree F H depth) (idx : Nat) (h : idx < 2 ^ depth):
+  MerkleTree.item_at_nat t idx = some a ↔
+  MerkleTree.tree_item_at_fin t ⟨idx, h⟩ = a := by
+  rw [item_at_nat_to_fin' (h := h)]
+  . simp
+
+theorem MerkleTree.item_at_fin_invariant' {H : Hash α 2} {tree tree': MerkleTree α H depth} {ix₁ ix₂ : Fin (2 ^ depth)} { neq : ix₁ ≠ ix₂ }:
+  MerkleTree.tree_set_at_fin tree ix₁ item₁ = tree' →
+  MerkleTree.tree_item_at_fin tree' ix₂ = MerkleTree.tree_item_at_fin tree ix₂ := by
+  rw [<-set_at_nat_to_fin_some' (h := ix₁.2)]
+  rw [<-item_at_nat_to_fin_some' (h := ix₂.2)]
+  rw [<-item_at_nat_to_fin' (h := ix₂.2)]
+  apply MerkleTree.item_at_nat_invariant (neq := fun h => neq (Fin.eq_of_veq h))
+
+lemma MerkleTree.item_at_fin_set_at_fin {H : Hash α 2} {tree : MerkleTree α H depth} {item: α} {ix: Fin (2 ^ depth)}:
+  tree_item_at_fin (tree.tree_set_at_fin ix item) ix = item := read_after_insert_sound _ _ _
+
+theorem ZMod.val_fin {n : ℕ } {f : ZMod n.succ}: f.val = Fin.val f := by
+  simp [val]
+
+
 -- Insertion round semantic equivalence
 
 def insertion_round (Path: Vector F D) (Item: F) (PrevRoot: F) (Proof: Vector F D) (k: F -> Prop) : Prop :=
@@ -26,64 +116,422 @@ def insertion_round_prep (Index: F) (Item: F) (PrevRoot: F) (Proof: Vector F D) 
   ∃out: Vector F D, recover_binary_zmod' out = Index ∧ is_vector_binary out ∧
   insertion_round out Item PrevRoot Proof k
 
-lemma InsertionRound_uncps {Index: F} {Item: F} {PrevRoot: F} {Proof: Vector F D} {k: F -> Prop} :
-  gInsertionRound Index Item PrevRoot Proof k ↔
-  insertion_round_prep Index Item PrevRoot Proof k := by
-  simp [insertion_round_prep, insertion_round]
-  simp [gInsertionRound]
+def fin_to_path (index : Nat) (d : Nat): Validate (index < 2^d) ⊕ Vector Dir d :=
+  if h : index < 2 ^ d then
+    Sum.inr (Dir.fin_to_dir_vec ⟨index, h⟩).reverse
+  else
+    Sum.inl ⟨h⟩
+
+def tree_proof_at_validate (tree : MerkleTree α H d) (index : Nat): Validate (index < 2 ^ d) ⊕ Vector α d := do
+  let p ← fin_to_path index d
+  pure $ tree.proof p
+
+def insertionRound_semantics (Index Item : F) (Tree : MerkleTree F poseidon₂ D) (Proof : Vector F D) (k : MerkleTree F poseidon₂ D → Prop): Prop :=
+  if h : Index.val < 2 ^ D then
+    Tree.tree_item_at_fin ⟨Index.val, h⟩ = 0 ∧
+    Tree.tree_proof_at_fin ⟨Index.val, h⟩ = Proof.reverse ∧
+    k (Tree.tree_set_at_fin ⟨Index.val, h⟩ Item)
+  else False
+
+lemma Fin.castNat_lt_pow {n k : ℕ} (h : n < 2^k) : ↑n = Fin.mk n h := by
+  apply Fin.eq_of_veq
+  exact Nat.mod_eq_of_lt h
+
+theorem insertionRound_rw [Fact (CollisionResistant poseidon₂)] {Tree : MerkleTree F poseidon₂ D} :
+  gInsertionRound Index Item Tree.root Proof k ↔
+  insertionRound_semantics Index Item Tree Proof (fun t => k t.root) := by
+  simp [insertionRound_semantics, gInsertionRound]
   simp [Gates.to_binary, Gates.eq]
   simp [VerifyProof_looped, proof_rounds_uncps]
-  simp [and_assoc]
-  apply exists_congr
-  intros
-  simp [double_prop]
-  rename_i gate
-  rw [←Vector.ofFn_get (v := gate)]
-  rw [←Vector.ofFn_get (v := Proof)]
-  tauto
-
-def insertion_rounds {n} (StartIndex: F) (PreRoot: F) (IdComms: Vector F n) (MerkleProofs: Vector (Vector F D) n) (k : F -> Prop) : Prop :=
-  match n with
-  | Nat.zero => k PreRoot
-  | Nat.succ _ => gInsertionRound StartIndex IdComms.head PreRoot MerkleProofs.head fun next =>
-    insertion_rounds (StartIndex + 1) next IdComms.tail MerkleProofs.tail k
-
-def InsertionLoop {n} (StartIndex: F) (PreRoot: F) (IdComms: Vector F n) (MerkleProofs: Vector (Vector F D) n) (k : F -> Prop) : Prop :=
-  match n with
-  | Nat.zero => k PreRoot
-  | Nat.succ _ =>
-    insertion_round_prep StartIndex IdComms.head PreRoot MerkleProofs.head fun next =>
-    InsertionLoop (StartIndex + 1) next IdComms.tail MerkleProofs.tail k
-
-lemma insertion_rounds_uncps {n} {StartIndex: F} {PreRoot: F} {IdComms: Vector F n} {MerkleProofs: Vector (Vector F D) n} {k : F -> Prop}:
-  insertion_rounds StartIndex PreRoot IdComms MerkleProofs k ↔
-  InsertionLoop StartIndex PreRoot IdComms MerkleProofs k := by
-  induction IdComms, MerkleProofs using Vector.inductionOn₂ generalizing StartIndex PreRoot with
-  | nil =>
-    unfold insertion_rounds
-    unfold InsertionLoop
-    rfl
-  | cons =>
-    unfold insertion_rounds
-    unfold InsertionLoop
-    simp [InsertionRound_uncps, insertion_round_prep, insertion_round]
-    rename_i ih
-    simp [ih]
-
-lemma InsertionProof_looped (StartIndex: F) (PreRoot: F) (IdComms: Vector F B) (MerkleProofs: Vector (Vector F D) B) (k: F -> Prop) :
-    gInsertionProof StartIndex PreRoot IdComms MerkleProofs k =
-      insertion_rounds StartIndex PreRoot IdComms MerkleProofs k := by
-        unfold gInsertionProof
-        simp [insertion_rounds]
-        simp [InsertionRound_uncps]
-        simp [Gates.add]
-        rw [add_assoc]
-        rw [add_assoc]
-        rw [←Vector.ofFn_get (v := IdComms)]
-        rw [←Vector.ofFn_get (v := MerkleProofs)]
+  apply Iff.intro
+  . intro ⟨path, ⟨path_rec, path_bin⟩, _, hpre, _, hpost⟩
+    split
+    . rename_i h
+      unfold MerkleTree.tree_item_at_fin
+      unfold MerkleTree.tree_set_at_fin
+      unfold MerkleTree.tree_proof_at_fin
+      simp_rw [←Fin.castNat_lt_pow h, Dir.recover_binary_zmod'_to_dir h (by decide) path_bin path_rec]
+      have : MerkleTree.recover poseidon₂ (Dir.create_dir_vec path).reverse Proof.reverse 0 = Tree.root := by
+        rw [←MerkleTree.recover_tail_equals_recover_reverse, ←hpre, ←Vector.ofFn_get (v := Proof)]
         rfl
+      refine ⟨?_, ?_, ?_⟩
+      . apply MerkleTree.proof_ceritfies_item
+        exact this
+      . apply MerkleTree.recover_proof_reversible
+        exact this
+      . rw [←MerkleTree.proof_insert_invariant, ←MerkleTree.recover_tail_equals_recover_reverse]
+        exact hpost
+        rotate_left
+        rw [←Vector.ofFn_get (v := Proof)] at this
+        exact this
+    . rename_i h
+      rw [recover_binary_zmod_bit path_bin] at path_rec
+      rw [←path_rec] at h
+      rw [binary_zmod_same_as_nat _ (by decide)] at h
+      exact h (binary_nat_lt _)
+  . intro hp
+    split at hp <;> try contradiction
+    rcases hp with ⟨hitem, hproof, hnext⟩
+    rename_i h
+    apply Exists.intro (Vector.map Bit.toZMod (fin_to_bits_le ⟨Index.val, h⟩))
+    simp only
+      [ ←Dir.recover_binary_zmod'_to_dir h (by decide) vector_binary_of_bit_to_zmod (fin_to_bits_recover_binary _ _)
+      , vector_binary_of_bit_to_zmod
+      , fin_to_bits_recover_binary _ _
+      , true_and
+      ]
+    unfold MerkleTree.tree_item_at_fin at hitem
+    unfold MerkleTree.tree_set_at_fin at hnext
+    unfold MerkleTree.tree_proof_at_fin at hproof
+    simp_rw [←Fin.castNat_lt_pow h] at hitem hnext hproof
+    refine ⟨?_, ?_⟩
+    . rw [MerkleTree.recover_tail_equals_recover_reverse]
+      rw [←MerkleTree.recover_equivalence]
+      refine ⟨hitem, ?_⟩
+      rw [hproof, ←Vector.ofFn_get (v := Proof)]
+      rfl
+    . apply Eq.subst _ hnext
+      rw [MerkleTree.recover_tail_equals_recover_reverse, eq_comm, ←MerkleTree.recover_equivalence]
+      refine ⟨MerkleTree.read_after_insert_sound _ _ _, ?_⟩
+      rw [MerkleTree.proof_of_set_is_proof, hproof, ←Vector.ofFn_get (v := Proof)]
+      rfl
 
-lemma InsertionProof_uncps {StartIndex: F} {PreRoot: F} {IdComms: Vector F B} {MerkleProofs: Vector (Vector F D) B} {k: F -> Prop}:
-    gInsertionProof StartIndex PreRoot IdComms MerkleProofs k ↔
-    InsertionLoop StartIndex PreRoot IdComms MerkleProofs k := by
-    simp only [InsertionProof_looped, insertion_rounds_uncps]
+def insertionRoundsSemantics {b : Nat}
+  (startIndex : F)
+  (tree : MerkleTree F poseidon₂ D)
+  (identities : Vector F b)
+  (proofs : Vector (Vector F D) b)
+  (k : F → Prop): Prop := match b with
+  | 0 => k tree.root
+  | Nat.succ _ => insertionRound_semantics
+      startIndex
+      identities.head
+      tree
+      proofs.head
+      fun t => insertionRoundsSemantics (startIndex + 1) t identities.tail proofs.tail k
+
+theorem exists_binder {f : α → Prop} : (∃x, x = y ∧ f x) ↔ f y := by
+  apply Iff.intro
+  . intro ⟨x, ⟨hx, hfx⟩⟩
+    rw [←hx]
+    exact hfx
+  . intro hfy
+    refine ⟨y, ⟨rfl, hfy⟩⟩
+
+theorem insertionRounds_rw [Fact (CollisionResistant poseidon₂)]  {Tree : MerkleTree F poseidon₂ D}:
+  gInsertionProof startIndex Tree.root idComms merkleProofs k ↔
+  insertionRoundsSemantics startIndex Tree idComms merkleProofs k := by
+  unfold gInsertionProof
+  simp_rw [insertionRound_rw, Gates.add, exists_binder]
+  apply Iff.of_eq
+  simp only [add_zero]
+
+  repeat (
+    unfold insertionRoundsSemantics
+    cases idComms using Vector.casesOn; rename_i idComm idComms -- with | cons idComm idComms =>
+    cases merkleProofs using Vector.casesOn; rename_i merkleProof merkleProofs
+    try rw [add_assoc]
+    congr
+    ext
+    apply Iff.of_eq
+  )
+
+  unfold insertionRoundsSemantics
+  cases idComms using Vector.casesOn with | cons idComm idComms =>
+  cases merkleProofs using Vector.casesOn with | cons merkleProof merkleProofs =>
+  try rw [add_assoc]
+  congr
+
+def rootTransformationSpec'' {B : ℕ}
+  (tree : MerkleTree F poseidon₂ D)
+  (identities : Vector F B)
+  (startIndex : Nat): Option (MerkleTree F poseidon₂ D) := match B with
+  | 0 => some tree
+  | _ + 1 => match tree.set_at_nat startIndex identities.head with
+    | some nextTree => rootTransformationSpec'' nextTree identities.tail (startIndex + 1)
+    | none => none
+
+lemma rootTransformSpec_some_ix_bound {B : ℕ} {identities : Vector F B.succ}:
+  rootTransformationSpec'' tree identities startIndex = some tree' →
+  startIndex < 2 ^ D := by
+  intro hp
+  conv at hp => lhs; whnf
+  split at hp
+  . apply MerkleTree.set_at_nat_some_when_le
+    assumption
+  . contradiction
+
+lemma rootTransformSpec_succ {B : ℕ} {identities : Vector F B.succ}
+  (hp : rootTransformationSpec'' tree identities startIndex = some tree'):
+  rootTransformationSpec''
+    (tree.tree_set_at_fin ⟨startIndex, rootTransformSpec_some_ix_bound hp⟩ identities.head)
+    identities.tail
+    (startIndex + 1) = some tree' := by
+    have bound : startIndex < 2 ^ D := rootTransformSpec_some_ix_bound hp
+    conv at hp => lhs; whnf
+    split at hp
+    . rename_i h
+      rw [MerkleTree.set_at_nat_to_fin' (h:=bound)] at h
+      injection h with h
+      rwa [h]
+    . contradiction
+
+theorem insertionRoundsRootTransformation
+  {B : ℕ} {startIndex : Nat} {identities : Vector F B} {proofs : Vector (Vector F D) B}
+  (indexIsValid : startIndex + B < 2 ^ D):
+  insertionRoundsSemantics startIndex tree identities proofs k →
+  ∃postTree, rootTransformationSpec'' tree identities startIndex = some postTree ∧ k postTree.root := by
+  intro hp
+  induction B generalizing startIndex tree with
+  | zero => exists tree
+  | succ B ih =>
+    unfold insertionRoundsSemantics at hp
+    unfold insertionRound_semantics at hp
+    split at hp
+    . rename_i bound
+      rcases hp with ⟨-, -, hp⟩
+      have := by
+        refine ih ?_ hp
+        rw [add_assoc]
+        apply Nat.lt_of_le_of_lt
+        . apply Nat.add_le_add_right
+          apply Nat.mod_le
+        . simp; linarith
+      have ixLeOrd : startIndex < Order := by
+        apply LT.lt.trans
+        apply Nat.lt_sub_of_add_lt
+        exact indexIsValid
+        apply Nat.lt_of_le_of_lt
+        apply Nat.sub_le
+        decide
+      rcases this with ⟨t, hsome, hk⟩
+      exists t
+      conv => arg 1; lhs; whnf
+      rw [MerkleTree.set_at_nat_to_fin']
+      simp
+      apply And.intro
+      . rw [←hsome]
+        congr
+        . exact Eq.symm (ZMod.val_cast_of_lt ixLeOrd)
+        . exact Eq.symm (Nat.mod_eq_of_lt ixLeOrd)
+        . rw [ZMod.val_cast_of_lt ixLeOrd] at bound; exact bound
+      . exact hk
+    . contradiction
+
+theorem insertionRoundsRootTransformation'
+  {B : ℕ} {startIndex : F} {identities : Vector F B} {proofs : Vector (Vector F D) B}:
+  -- (indexIsValid : startIndex + B < 2 ^ D):
+  insertionRoundsSemantics startIndex tree identities proofs k →
+  ∃postTree, rootTransformationSpec'' tree identities startIndex.val = some postTree ∧ k postTree.root := by
+  intro hp
+  induction B generalizing startIndex tree with
+  | zero => exists tree
+  | succ B ih =>
+    unfold insertionRoundsSemantics at hp
+    unfold insertionRound_semantics at hp
+    split at hp
+    . rename_i bound
+      rcases hp with ⟨-, -, hp⟩
+      have := ih hp
+        -- refine ih hp
+        -- rw [add_assoc]
+        -- apply Nat.lt_of_le_of_lt
+        -- . apply Nat.add_le_add_right
+        --   apply Nat.mod_le
+        -- . simp; linarith
+      -- have ixLeOrd : startIndex < Order := by
+      --   apply LT.lt.trans
+      --   apply Nat.lt_sub_of_add_lt
+      --   exact indexIsValid
+      --   apply Nat.lt_of_le_of_lt
+      --   apply Nat.sub_le
+      --   decide
+      rcases this with ⟨t, hsome, hk⟩
+      exists t
+      conv => arg 1; lhs; whnf
+      rw [MerkleTree.set_at_nat_to_fin']
+      simp
+      apply And.intro
+      . rw [←hsome]
+        congr
+        . exact Eq.symm (ZMod.val_cast_of_lt ixLeOrd)
+        . exact Eq.symm (Nat.mod_eq_of_lt ixLeOrd)
+        . rw [ZMod.val_cast_of_lt ixLeOrd] at bound; exact bound
+      . exact hk
+    . contradiction
+
+theorem before_insertion_all_zero
+  {B: ℕ} {startIndex : F} {proofs : Vector (Vector F D) B} {identities : Vector F B}:
+  insertionRoundsSemantics (b := B) startIndex tree identities proofs k →
+  ∀i ∈ [startIndex.val : (startIndex + B).val], tree.item_at_nat i = some 0 := by
+  intro hp i hi
+
+  induction B generalizing i startIndex tree with
+  | zero =>
+    cases hi; rename_i hl hu
+    simp at hu
+    simp at hl
+    have := Nat.lt_of_le_of_lt hl hu
+    have := lt_irrefl _ this
+    contradiction
+  | succ B ih =>
+    cases identities using Vector.casesOn with | cons id ids =>
+    cases proofs using Vector.casesOn with | cons proof proofs =>
+    unfold insertionRoundsSemantics at hp
+    unfold insertionRound_semantics at hp
+    rcases hi with ⟨hil, hiu⟩
+    split at hp
+    . cases hil
+      . rcases hp with ⟨hp, -, -⟩
+        rename_i h
+        rw [MerkleTree.item_at_nat_to_fin', hp]
+      . rename_i i hil
+        rcases hp with ⟨-, -, hp⟩
+        have := ih hp (i.succ) (by
+          apply And.intro
+          . apply Nat.le_trans (m := startIndex.val + 1)
+            simp [ZMod.val_fin]
+            rw [Fin.val_add_one]
+            split <;> simp
+            simp_arith
+            assumption
+          . apply Nat.lt_of_lt_of_eq hiu
+            simp [add_assoc]
+            rw [add_comm (b:=1)]
+        )
+        have bound := MerkleTree.item_at_nat_some_when_le this
+        rw [MerkleTree.item_at_nat_to_fin' _ _ bound] at this
+        rw [MerkleTree.item_at_fin_invariant'] at this
+        rw [←MerkleTree.item_at_nat_to_fin' _ _ bound] at this
+        assumption
+        rfl
+        simp
+        apply Nat.ne_of_lt
+        apply Nat.lt_succ_of_le
+        assumption
+    . contradiction
+
+theorem ix_bound {B : ℕ} {startIndex : F} {identities : Vector F B.succ} {proofs : Vector (Vector F D) B.succ}:
+  insertionRoundsSemantics startIndex tree identities proofs k →
+  startIndex.val + B < 2 ^ D := by
+  induction B generalizing startIndex tree with
+  | zero =>
+    intro hp
+    unfold insertionRoundsSemantics at hp
+    unfold insertionRound_semantics at hp
+    split at hp
+    . simpa
+    . contradiction
+  | succ B ih =>
+    intro hp
+    unfold insertionRoundsSemantics at hp
+    unfold insertionRound_semantics at hp
+    split at hp
+    . rename_i hi
+      rcases hp with ⟨-, -, hp⟩
+      have := ih hp
+      rw [ZMod.val_fin] at this hi
+      cases identities using Vector.casesOn with | cons id ids =>
+      cases proofs using Vector.casesOn with | cons proof proofs =>
+      rw [Fin.val_add_one_of_lt _] at this
+      . rw [ZMod.val_fin]
+        linarith
+      . rw [Fin.lt_iff_val_lt_val]
+        exact LT.lt.trans hi (by decide)
+    . contradiction
+
+instance : Decidable (i ∈ [a : b]) := by
+  simp [Membership.mem]; infer_instance
+
+lemma treeTransform_get_lt {i : Nat} {B : ℕ} {startIndex : Nat}
+  {identities : Vector F B}:
+  rootTransformationSpec'' tree identities startIndex = some tree' →
+  i < startIndex → tree.item_at_nat i = tree'.item_at_nat i := by
+  induction B generalizing startIndex tree tree' with
+  | zero =>
+    intro h _
+    cases identities using Vector.casesOn
+    injection h with h
+    rw [h]
+  | succ B ih =>
+    intro h hu
+    cases identities using Vector.casesOn
+    conv at h => lhs; whnf
+    split at h
+    . rename_i hp'
+      have := ih h (by linarith)
+      rw [←this]
+      have sibound : startIndex < 2^D := MerkleTree.set_at_nat_some_when_le hp'
+      have ibound : i < 2^D := lt_trans hu sibound
+      rw [MerkleTree.set_at_nat_to_fin_some' (h:=sibound)] at hp'
+      rw [MerkleTree.item_at_nat_to_fin' (h:=ibound)]
+      rw [MerkleTree.item_at_nat_to_fin' (h:=ibound)]
+      apply congrArg
+      apply Eq.symm
+      apply MerkleTree.item_at_fin_invariant' hp'
+      intro hp
+      injection hp with hp
+      exact Nat.ne_of_lt hu (eq_comm.mp hp)
+    . contradiction
+
+lemma treeTransform_get_gt {i B startIndex : ℕ}
+  {identities : Vector F B}:
+  rootTransformationSpec'' tree identities startIndex = some tree' →
+  i ≥ startIndex + B → tree.item_at_nat i = tree'.item_at_nat i := by
+  induction B generalizing startIndex tree tree' with
+  | zero =>
+    intro h _
+    cases identities using Vector.casesOn
+    injection h with h
+    rw [h]
+  | succ B ih =>
+    intro h hl
+    cases identities using Vector.casesOn
+    conv at h => lhs; whnf
+    split at h
+    . cases Nat.lt_or_ge i (2^D) with
+      | inl ibound =>
+        rename_i hp
+        have sibound : startIndex < 2^D := MerkleTree.set_at_nat_some_when_le hp
+        repeat rw [MerkleTree.item_at_nat_to_fin' (h:=ibound)]
+        rw [MerkleTree.set_at_nat_to_fin_some' (h:=sibound)] at hp
+        have := ih h (by linarith)
+        repeat rw [MerkleTree.item_at_nat_to_fin' (h:=ibound)] at this
+        rw [←this]
+        apply congrArg
+        apply Eq.symm
+        apply MerkleTree.item_at_fin_invariant' hp
+        intro hp
+        injection hp with hp
+        linarith
+      | inr h =>
+        simp_rw [MerkleTree.item_at_nat_none_when_ge h]
+    . contradiction
+
+lemma treeTransform_get_inrange {i B startIndex : ℕ} {identities : Vector F B}
+  (hp : rootTransformationSpec'' tree identities startIndex = some tree')
+  (inrange : i ∈ [0 : B]):
+  tree'.item_at_nat (startIndex + i) = identities[i]'inrange.2 := by
+  induction B generalizing startIndex i tree tree' with
+  | zero => cases inrange; exfalso; linarith
+  | succ B ih =>
+    have := rootTransformSpec_succ hp
+    have bound := rootTransformSpec_some_ix_bound hp
+    cases identities using Vector.casesOn with | cons id ids =>
+    cases i with
+    | zero =>
+      have := treeTransform_get_lt this (by linarith)
+      simp
+      rw [←this, MerkleTree.item_at_nat_to_fin_some' _ _ bound]
+      simp
+      apply MerkleTree.read_after_insert_sound
+    | succ i =>
+      have inrange : i ∈ [0 : B] := by
+        cases inrange
+        apply And.intro <;> linarith
+      have := ih this inrange
+      simp
+      simp at this
+      rw [←this]
+      apply congrArg
+      simp_arith
