formal-verification/Main.lean
@@ -8,6 +8,7 @@ import FormalVerification.Utils
 import FormalVerification.Poseidon.Spec
 import FormalVerification.Poseidon.Correctness
 import FormalVerification.Keccak.SemanticEquivalence
+import FormalVerification.KeccakUniqueness
 import FormalVerification.BinaryReps.Basic
 import FormalVerification.BinaryReps.SemanticEquivalence
 
@@ -18,6 +19,172 @@ import FormalVerification.InsertionCircuit
 import FormalVerification.DeletionCircuit
 
 open SemaphoreMTB (F Order)
+
+instance : Membership α (Vector α n) := ⟨fun x xs => x ∈ xs.toList⟩
+
+namespace MerkleTree
+
+instance : GetElem (MerkleTree α H d) Nat α (fun _ i => i < 2^d) where
+  getElem tree ix inb := tree.tree_item_at_fin ⟨ix, inb⟩
+
+lemma getElem?_eq_item_at_nat {d} (tree : MerkleTree α H d) (ix : Nat) :
+  tree[ix]? = tree.item_at_nat ix := by
+  simp only [getElem?, getElem]
+  split
+  . rename_i h
+    rw [eq_comm, MerkleTree.item_at_nat_to_fin_some']
+  . rename_i h
+    exact eq_comm.mp (MerkleTree.item_at_nat_none_when_ge (Nat.ge_of_not_lt h))
+
+lemma getElem!_eq_item_at_nat [Inhabited α] {d} {tree : MerkleTree α H d} {ix : ℕ}:
+  tree[ix]! = (tree.item_at_nat ix).get! := by
+  simp only [getElem!, getElem]
+  split
+  . rename_i h
+    rw [eq_comm, MerkleTree.item_at_nat_to_fin' (h:=h)]
+    rfl
+  . rename_i h
+    rw [MerkleTree.item_at_nat_none_when_ge (Nat.ge_of_not_lt h)]
+    conv => lhs; whnf
+
+end MerkleTree
+
+namespace Deletion
+
+/-!
+### Input Hash Correctness
+
+Both Semaphore MTB circuits use a construction where the inputs that are
+logically used as public inputs, are instead concatenated and hashed to a single
+field element. This hash is the only real public input to the circuit. This is
+done to significantly reduce the cost of proof verification.
+
+This section establishes the correctness of that construction.
+-/
+section InputHash
+
+/--
+Establishes that the deletion circuit's InputHash parameter is uniquely
+determined by DeletionIndices, PreRoot and PostRoot. That is done by showing
+that any two valid assigments that agree on those parameters, must also agree
+on InputHash.
+-/
+theorem DeletionCircuit_InputHash_deterministic:
+  (SemaphoreMTB.DeletionMbuCircuit_4_4_30_4_4_30 InputHash₁ DeletionIndices PreRoot PostRoot IdComms₁ MerkleProofs₁ ∧
+   SemaphoreMTB.DeletionMbuCircuit_4_4_30_4_4_30 InputHash₂ DeletionIndices PreRoot PostRoot IdComms₂ MerkleProofs₂)
+  → InputHash₁ = InputHash₂
+  := Deletion_InputHash_deterministic
+
+/--
+Establishes that the insertion circuit's InputHash parameter is uniquely
+determined by StartIndex, PreRoot, PostRoot and the identity commitments. That
+is done by showing that any two valid assigments that agree on those
+parameters, must also agree on InputHash.
+-/
+theorem InsertionCircuit_InputHash_deterministic:
+  SemaphoreMTB.InsertionMbuCircuit_4_30_4_4_30 InputHash₁ StartIndex PreRoot PostRoot IdComms MerkleProofs₁ ∧
+  SemaphoreMTB.InsertionMbuCircuit_4_30_4_4_30 InputHash₂ StartIndex PreRoot PostRoot IdComms MerkleProofs₂ →
+  InputHash₁ = InputHash₂
+  := Insertion_InputHash_deterministic
+
+
+end InputHash
+
+section InputValidations
+
+theorem indices_rangecheck:
+  SemaphoreMTB.DeletionMbuCircuit_4_4_30_4_4_30 InputHash DeletionIndices PreRoot PostRoot IdComms MerkleProofs →
+  ∀ v ∈ DeletionIndices, v.val < 2^32 := by
+  intro hp v hv
+  have hp := Deletion_skipHashing hp
+  sorry
+
+end InputValidations
+
+
+end Deletion
+
+namespace Insertion
+
+section InputValidations
+
+theorem before_insertion_all_items_zero
+  [Fact (CollisionResistant poseidon₂)]
+  {tree: MerkleTree F poseidon₂ D}
+  {startIndex : F}:
+  SemaphoreMTB.InsertionMbuCircuit_4_30_4_4_30 InputHash startIndex tree.root PostRoot IdComms MerkleProofs →
+  ∀ i ∈ [startIndex.val:startIndex.val + B], tree[i]! = 0 := by
+  intro hp i hir
+  have hp := Insertion_skipHashing hp
+  rw [insertionRounds_rw] at hp
+  have hp'' := ix_bound hp
+  rw [MerkleTree.getElem!_eq_item_at_nat]
+  rw [before_insertion_all_zero hp]; rfl
+  apply And.intro
+  . exact hir.1
+  . apply Nat.lt_of_lt_of_eq hir.2
+    rw [ZMod.val_add, Nat.mod_eq_of_lt]
+    rfl
+    calc
+      startIndex.val + 4 = (startIndex.val + 3) + 1 := by ring
+      _ < 2^D + 1 := Nat.add_lt_add_right hp'' (k := 1)
+      _ < Order := by decide
+
+end InputValidations
+
+
+section Semantics
+
+theorem root_transformation_correct
+  [Fact (CollisionResistant poseidon₂)]
+  {StartIndex : ℕ}
+  {Tree : MerkleTree F poseidon₂ D}:
+  SemaphoreMTB.InsertionMbuCircuit_4_30_4_4_30 InputHash StartIndex Tree.root PostRoot IdComms MerkleProofs →
+  ∃(postTree : MerkleTree F poseidon₂ D),
+  postTree.root = PostRoot ∧
+  (∀ i, i ∈ [StartIndex:StartIndex + B] → postTree[i]! = IdComms[i-StartIndex]!) ∧
+  (∀ i, i ∉ [StartIndex:StartIndex + B] → postTree[i]! = Tree[i]!) := by
+  intro hp
+  have hp := Insertion_skipHashing hp
+  rw [insertionRounds_rw] at hp
+  have hp := insertionRoundsRootTransformation (by sorry) hp
+
+
+
+def rootTransformationSpec
+  (tree : MerkleTree F poseidon₂ D)
+  (identities : Vector F B)
+  (startIndex : Nat)
+  (indexIsValid : startIndex + B < 2 ^ D): MerkleTree F poseidon₂ D := Id.run do
+  let mut tree := tree
+  for h : i in [0 : B] do
+    have i_valid : startIndex + i < 2 ^ D :=
+      Nat.lt_of_lt_of_le (Nat.add_lt_add_left h.2 _) (le_of_lt indexIsValid)
+    tree := tree.tree_set_at_fin ⟨startIndex + i, i_valid⟩ (identities[i]'h.2)
+  tree
+
+theorem rootTransformationSpec_correct
+  [Fact (CollisionResistant poseidon₂)]
+  {Tree : MerkleTree F poseidon₂ D}
+  (index_valid : StartIndex + B < 2 ^ D):
+  SemaphoreMTB.InsertionMbuCircuit_4_30_4_4_30 InputHash StartIndex Tree.root PostRoot IdComms MerkleProofs →
+  PostRoot = (rootTransformationSpec Tree IdComms StartIndex index_valid).root := by
+  intro hp
+  have hp := Insertion_skipHashing hp
+  rw [insertionRounds_rw, InsertionLoop, insertion_round_prep] at hp
+  rcases hp with ⟨_, _, _, hp⟩
+
+
+
+
+
+
+end Semantics
+
+
+end Insertion
+
+-- def treeInsertionSpec {d b} (tree : MerkleTree F poseidon₂ d)
 
 theorem insertion_is_set_circuit
   [Fact (CollisionResistant poseidon₂)]
